FY/Assertion.v
@@ -23,5 +23,8 @@ Fixpoint Expectation (ns na : nat)
     end
 .
 
-Definition weaker (ns na1 na2 : nat) (state: list ((total_map nat)*(Unitary ns))) (assertion1: Assertion na1) (assertion2: Assertion na2) : Prop :=
+Definition weaker (ns na1 na2 : nat) 
+    (state: list ((total_map nat)*(Unitary ns))) 
+    (assertion1: Assertion na1) 
+    (assertion2: Assertion na2) : Prop :=
     Cnorm (Expectation ns na1 state assertion1) <= Cnorm (Expectation ns na2 state assertion2).
