FY/Teleportation.v
@@ -12,20 +12,20 @@ Definition X1 : string := "X1".
 
 Definition TELEPORT : com :=
   <{ 
-     q 0 := 0;
-     q 1 := 0;
-     q 2 := 0;
-     q 1 *=1 GH;
-     q 1 2 *=2 GCNOT;
-     q 0 1 *=2 GCNOT;
-     q 0 *=1 GH;
-     X0 :=measQ 0;
-     X1 :=measQ 1;
+     new_qubit;
+     new_qubit;
+     new_qubit;
+     q 1 *= GH;
+     q 1 2 *= GCNOT;
+     q 0 1 *= GCNOT;
+     q 0 *= GH;
+     X0 :=meas 0;
+     X1 :=meas 1;
      if X0 == (0 % nat)
      then 
-       if X1 == (1 % nat) then q 2 *=1 GX else skip end 
+       if X1 == (1 % nat) then q 2 *= GX else skip end 
      else
-       if X1 == (1 % nat) then q 2 *=1 GX; q 2 *=1 GZ else q 2 *=1 GZ end 
+       if X1 == (1 % nat) then q 2 *= GX; q 2 *= GZ else q 2 *= GZ end 
      end
   }>.
 
@@ -85,7 +85,7 @@ ket1 = np.array([0,1])
 
 init = np.kron(ket0, np.kron(ket0, ket0)).reshape(-1,1)
 
-fst = init.dot(init.T)
+fst = init.dot(init.T) 
 #print(fst)
 
 u1 = np.kron(H, np.kron(I, I))
